RocqOfRust/revm/revm_interpreter/instructions/links/arithmetic.v
@@ -9,7 +9,7 @@ Require Import revm.revm_interpreter.links.instruction_result.
 Require Import revm.revm_interpreter.links.interpreter.
 Require Import revm.revm_interpreter.links.interpreter_types.
 Require Import revm.revm_interpreter.instructions.links.i256.
-Require Import revm.revm_specification.links.hardfork.
+Require Import revm.revm_primitives.links.hardfork.
 Require Import ruint.links.add.
 Require Import ruint.links.bits.
 Require Import ruint.links.cmp.
