RocqOfRust/revm/revm_interpreter/instructions/links/memory/mstore.v
@@ -10,10 +10,11 @@ Require Import revm.revm_interpreter.gas.links.constants.
 Require Import revm.revm_interpreter.instructions.memory.
 Require Import revm.revm_interpreter.interpreter.links.shared_memory.
 Require Import revm.revm_interpreter.links.gas.
+Require Import revm.revm_interpreter.links.instruction_context.
 Require Import revm.revm_interpreter.links.instruction_result.
 Require Import revm.revm_interpreter.links.interpreter.
 Require Import revm.revm_interpreter.links.interpreter_types.
-Require Import revm.revm_specification.links.hardfork.
+Require Import revm.revm_primitives.links.hardfork.
 Require Import ruint.links.bits.
 Require Import ruint.links.bytes.
 Require Import ruint.links.from.
@@ -24,18 +25,20 @@ Instance run_mstore
   {WIRE_types : InterpreterTypes.Types.t} `{InterpreterTypes.Types.AreLinks WIRE_types}
   {H_types : Host.Types.t} `{Host.Types.AreLinks H_types}
   (run_InterpreterTypes_for_WIRE : InterpreterTypes.Run WIRE WIRE_types)
-  (interpreter : '&mut (Interpreter.t WIRE WIRE_types)) 
-  (host : '&mut H) :
+  (context : InstructionContext.t H WIRE WIRE_types) :
   Run.Trait
-    instructions.memory.mstore [] [ Φ WIRE; Φ H ] [ φ interpreter; φ host ]
+    instructions.memory.mstore [] [ Φ WIRE; Φ H ] [ φ context ]
     unit.
 Proof.
   constructor.
-  destruct run_InterpreterTypes_for_WIRE.
+  destruct run_InterpreterTypes_for_WIRE eqn:?.
   destruct run_LoopControl_for_Control.
   destruct run_StackTrait_for_Stack.
   destruct run_RuntimeFlag_for_RuntimeFlag.
   destruct run_MemoryTrait_for_Memory.
   run_symbolic.
+  all: eapply Impl_Interpreter.run_halt_memory_oog ||
+       eapply Impl_Interpreter.run_halt_underflow ||
+       eapply Impl_Interpreter.run_halt.
 Defined.
 Global Opaque run_mstore.
