RocqOfRust/revm/revm_interpreter/instructions/links/system/codesize.v
@@ -26,7 +26,7 @@ Require Import revm.revm_interpreter.links.instruction_result.
 Require Import revm.revm_interpreter.links.interpreter.
 Require Import revm.revm_interpreter.links.interpreter_types.
 Require Import revm.revm_primitives.links.lib.
-Require Import revm.revm_specification.links.hardfork.
+Require Import revm.revm_primitives.links.hardfork.
 Require Import ruint.links.from.
 Require Import ruint.links.lib.
 
