RocqOfRust/revm/revm_interpreter/instructions/simulate/contract/call_code.v
@@ -15,8 +15,8 @@ Require Import revm.revm_interpreter.instructions.simulate.macros.
 Require Import revm.revm_interpreter.links.interpreter.
 Require Import revm.revm_interpreter.links.interpreter_types.
 Require Import revm.revm_interpreter.simulate.interpreter_types.
-Require Import revm.revm_specification.links.hardfork.
-Require Import revm.revm_specification.simulate.hardfork.
+Require Import revm.revm_primitives.links.hardfork.
+Require Import revm.revm_primitives.simulate.hardfork.
 Require Import ruint.simulate.cmp.
 Require Import ruint.simulate.from.
 Require Import ruint.simulate.lib.
