RocqOfRust/revm/revm_interpreter/instructions/simulate/host/selfbalance.v
@@ -11,7 +11,7 @@ Require Import revm.revm_interpreter.links.interpreter.
 Require Import revm.revm_interpreter.links.instruction_result.
 Require Import revm.revm_interpreter.links.interpreter_types.
 Require Import revm.revm_interpreter.simulate.interpreter_types.
-Require Import revm.revm_specification.links.hardfork.
+Require Import revm.revm_primitives.links.hardfork.
 
 Definition selfbalance
     {WIRE H : Set} `{Link WIRE} `{Link H}
