RocqOfRust/revm/revm_interpreter/instructions/simulate/system/returndatacopy.v
@@ -6,7 +6,7 @@ Require Import core.num.simulate.mod.
 Require Import revm.revm_interpreter.instructions.simulate.system.memory_resize.
 Require Import revm.revm_interpreter.instructions.links.system.returndatacopy.
 Require Import revm.revm_interpreter.instructions.simulate.macros.
-Require Import revm.revm_specification.links.hardfork.
+Require Import revm.revm_primitives.links.hardfork.
 Require Import revm.revm_interpreter.links.instruction_result.
 Require Import revm.revm_interpreter.links.interpreter.
 Require Import revm.revm_interpreter.links.interpreter_types.
